theories/tests/higher_order.v
@@ -10,11 +10,11 @@ Section example.
 
   Lemma higher_order_spec k ks E g Φ P Q:
     abs_spec g E P Q ∗ P ∗ (Q -∗ WP (fill_ectxs void k, ks) {{ Φ }})
-    ⊢ WP (fill_ectxs (Ecall Tvoid g []) k, ks) @ E {{ Φ }}.
+    ⊢ WP (fill_ectxs (Ecall Tvoid g Vvoid) k, ks) @ E {{ Φ }}.
   Proof.
     iIntros "(Hg & HP & HΦ)".
     iDestruct "Hg" as (e) "[Ht He]".
-    iApply (wp_call _ []); last iFrame; first done.
+    iApply (wp_call _ Vvoid); last iFrame; first done.
     iNext. iApply ("He" with "HP").
     iApply "HΦ".
   Qed.
