theories/tests/rec.v
@@ -8,7 +8,7 @@ Section proof.
     if: ("x" != 0)
     then: (
       "x" <- "x" - 1 ;;
-      Ecall Tvoid "g" [Evar "x"] ;;
+      Ecall Tvoid "g" (Epair (Evar "x") (Evalue Vvoid)) ;;
       return: void)
     else: ( return: void ).
 
@@ -16,41 +16,43 @@ Section proof.
     if: ("x" != 0)
     then: (
       "x" <- "x" - 1 ;;
-      Ecall Tvoid "f" [Evar "x"] ;;
+      Ecall Tvoid "f" (Epair (Evar "x") (Evalue Vvoid));;
       return: void)
     else: ( return: void ).
 
   Lemma rec_example (n: nat) k ks Φ:
     "f" T↦ Function Tvoid [("x", Tint32)] f ∗
     "g" T↦ Function Tvoid [("x", Tint32)] g ∗ Φ void
-    ⊢ WP (fill_ectxs (Ecall Tvoid "f" [Evalue (Vint32 n)]) k, ks) {{ Φ }}.
+    ⊢ WP (fill_ectxs (Ecall Tvoid "f"
+                            (Evalue (Vpair (Vint32 n) Vvoid))) k, ks) {{ Φ }}.
   Proof.
     iIntros "[#? [#? HΦ]]".
     iLöb as "IH" forall (n k ks Φ).
     destruct n eqn:?; subst.
     - admit. (* simple base case *)
-    - iApply (wp_call _ [Vint32 (S n0)]); last iFrame "#"; first done.
-    iNext. wp_alloc ln as "Hln".
-    wp_let. wp_load. wp_op.
-    { instantiate (1:=vtrue). admit. }
-    wp_step. iNext. wp_load. wp_op.
-    replace (Z.pos (Pos.of_succ_nat n0) - 1%Z)%int with (Int.repr n0); last admit.
-    wp_assign.
-    iApply (wp_bind [EKseq _; EKcall _ _ [] []])=>//.
-    wp_load. iApply wp_value=>//.
-    wp_unfill (Ecall _ _ _).
-    iApply (wp_call [EKseq (return: void)] [Vint32 n0]);
-      last iFrame "#"; first done.
-    iNext. wp_alloc lx as "Hlx".
-    wp_let. wp_load.
-    destruct n0 eqn:?; subst.
-    + admit.
-    + replace (S n != 0%Z)%E with (Evalue vtrue); last admit.
-      do 5 wp_step. wp_unfill (Ecall _ _ _)%E.
-      simpl.
-      replace (! lx @ Tint32)%E with
-      (Evalue $ (n - 1)); last admit. wp_unfill (Ecall _ _ _)%E.
-      iApply ("IH" $! (n - 1)). done.
+    - iApply (wp_call _ (Vpair (Vint32 (S n0)) Vvoid)); last iFrame "#"; first done.
+      iNext. wp_alloc ln as "Hln".
+      wp_let. wp_load. wp_op.
+      { instantiate (1:=vtrue). admit. }
+      wp_step. iNext. wp_load. wp_op.
+      replace (Z.pos (Pos.of_succ_nat n0) - 1%Z)%int with (Int.repr n0); last admit.
+      wp_assign.
+      iApply (wp_bind [EKseq _; EKcall _ _])=>//.
+      admit.
+      (* wp_load. iApply wp_value=>//. *)
+      (* wp_unfill (Ecall _ _ _). *)
+      (* iApply (wp_call [EKseq (return: void)] [Vint32 n0]); *)
+      (*   last iFrame "#"; first done. *)
+      (* iNext. wp_alloc lx as "Hlx". *)
+      (* wp_let. wp_load. *)
+      (* destruct n0 eqn:?; subst. *)
+      (* + admit. *)
+      (* + replace (S n != 0%Z)%E with (Evalue vtrue); last admit. *)
+      (*   do 5 wp_step. wp_unfill (Ecall _ _ _)%E. *)
+      (*   simpl. *)
+      (*   replace (! lx @ Tint32)%E with *)
+      (*   (Evalue $ (n - 1)); last admit. wp_unfill (Ecall _ _ _)%E. *)
+      (*   iApply ("IH" $! (n - 1)). done. *)
   Admitted.
     
 End proof.
