theories/tests/spawn.v
@@ -11,9 +11,9 @@ Section test.
   Definition R: iProp Σ := (∃ vx: int32, lx ↦ vx @ Tint32)%I.
   
   Definition add: expr :=
-    Ecall Tvoid "acquire" [Evalue l] ;;
+    Ecall Tvoid "acquire" (Evalue (Vpair l Vvoid)) ;;
     lx <- !lx@Tint32 + 1;;
-    Ecall Tvoid "release" [Evalue l].
+    Ecall Tvoid "release" (Evalue (Vpair l Vvoid)).
 
   Lemma add_safe ks:
     is_lock N γ l R ∗
@@ -36,8 +36,8 @@ Section test.
      by encoding some receipt tokens *)
 
   Definition spawn: expr :=
-    Efork Tvoid "add" [] ;;
-    Efork Tvoid "add" [].
+    Efork Tvoid "add" Vvoid ;;
+    Efork Tvoid "add" Vvoid.
 
   Lemma spawn_spec ks:
     is_lock N γ l R ∗
@@ -48,9 +48,9 @@ Section test.
   Proof.
     iIntros "(#Hlk & #? & #? & #?)".
     unfold spawn. iApply wp_seq=>//.
-    iApply (wp_fork _ _ _ []); last iFrame "#"; first done.
+    iApply (wp_fork _ _ _ Vvoid); last iFrame "#"; first done.
     iNext. iSplitL "".
-    - wp_skip. iApply (wp_fork _ _ _ []); last iFrame "#"; first done.
+    - wp_skip. iApply (wp_fork _ _ _ Vvoid); last iFrame "#"; first done.
       iNext. iSplit=>//. iApply add_safe. iFrame "#".
     - iApply add_safe. iFrame "#".
   Qed.
